

$$\begin{pmatrix} a_{11} & a_{12} & a_{13} & \dots & a_{1k} & \dots & a_{1n} & b_1 \\ a_{21} & a_{22} & a_{23} & \dots & a_{2k} & \dots & a_{2n} & b_2 \\ \vdots & \vdots & \vdots & \ddots & \vdots & \ddots & \vdots & \vdots \\ a_{m1} & a_{m2} & a_{m3} & \dots & a_{mk} & \dots & a_{mn} & b_m \end{pmatrix}$$

$$(2n+1)(n-1) \quad \sum_{i=1}^m i = \frac{m(m+1)}{2}$$

$$\sum_{i=1}^n (2n+1)(n-1) \quad \frac{m(m+1)(2m+1)}{6}$$

$$\sum_{i=1}^m i^2 = \frac{m(m+1)(2m+1)}{6}$$

$$\sum_{i=1}^{n-1} [2i^2 + (-4n-3)i + (2n^2+3n)]$$

$$2 \sum_{i=1}^{n-1} i^2 + (-4n-3) \sum_{i=1}^{n-1} i + (2n^2+3n) \sum_{i=1}^{n-1} 1 \quad m=n-1$$

$$2 \frac{m(m+1)(2m+1)}{6} + (-4n-3) \frac{m(m+1)}{2} + (2n^2+3n)m$$

$$2 \frac{m(2m^2+2m+m+1)}{6} + \frac{(-4n-3)(n-1)(n)}{2} + 2n^3+3n^2-2n^2-3n$$

$$2 \frac{(2m^3+2m^2+m^2+1)}{6} + \frac{(-4n-3)(n^2-n)}{2} + 2n^3+n^2-3n$$

$$\frac{2m^3+3m^2+1}{3} + \frac{-4n^3-3n^2-4n^2-3n}{2} + 2n^3+n^2-3n$$

$$\frac{(2n-1)^3+3(n-1)^2+1}{3} = \frac{2(n^3-3n^2+n-1)}{3} - \frac{4n^3-3n^2-4n^2-3n}{2} + 2n^3+n^2-3n$$

$$\begin{aligned} & (2n+1-i+1)(n-1) \\ &= (2n+2-2i+1)(n-1) \\ &= (2n+3-2i)(n-1) \\ &= 2n^2-2ni+3n-3i-2ni+2i^2 \\ &= 2n^2+2i^2+3n-3i-4ni \\ &= 2i^2+i(-4n-3)+2n^2+3n \end{aligned}$$

$$\frac{2n^3-3n^2+n-1}{3} - \frac{4n^3-3n^2-4n^2-3n}{2} + 2n^3+n^2-3n$$

$$\frac{2n^3}{3} = n^2 + \frac{n}{3} - \cancel{2n^3} + \frac{n^2}{2} + \frac{3n}{2} + \cancel{2n^3} + \cancel{n^2} - 3n$$

$$= \frac{2n^3}{3} + \frac{n^2}{2} - \frac{7n}{6}$$

Para la parte
le Gauss

Para Jordan $\sum_{i=1}^n 3(i-1)$

$$3 \left(\frac{(n-1)(n-1+1)}{2} - 1 \right)$$

$$3 \left(\frac{(n-1)(n)}{2} - 1 \right) = 3 \left(\frac{n^2 - n}{2} - 1 \right) = 3 \left(\frac{n^2 - n}{2} - 1 \right)$$

En clase vimos los
3 que se necesitan
para cada paso de
Jordan, por eso
son 3.

1	x	x	x	y	3+
2		x	x	y	3+
3			x	y	3+

$$\frac{3n^2}{2} - \frac{3n}{2} - 3$$